Grep bash-style. Falta tentar meter o sorted invariant no grep.

Part 2 - Dafny/grep-naive/grep.dfy
@@ -11,22 +11,36 @@ predicate inRange(i: int, len: int, j: int, len2: int) {
   0 <= i < len && 0 <= j < len2
 }
 
-method Grep(word: array<byte>, query: array<char>) returns (found: bool, indexes: seq<int>)
+predicate sorted(s: seq<nat>, diff: nat)
+{
+  forall i,j :: 0 <= i < j < |s| ==> s[i] <= s[j]
+}
+
+method Grep(word: array<char>, query: array<char>) returns (found: bool, indexes: seq<nat>)
 requires word.Length > 0
 requires query.Length > 0
+requires word.Length >= query.Length
+//ensures forall v :: 0 <= v < |indexes| ==> indexes[v] < word.Length
+ensures forall k :: 0 <= k < |indexes| ==> indexes[k] < word.Length
+ensures forall k :: 0 <= k < |indexes| ==> indexes[k] + query.Length <= word.Length
 {
-  var i, j, pos := 0, 0, 0;
+  var i, j, pos: nat := 0, 0, 0;
   indexes := [];
 
   while (i < word.Length) 
   invariant i <= word.Length
   invariant j < query.Length
   invariant j <= i
+  invariant 0 <= pos <= i - j
+  invariant forall k :: 0 <= k < |indexes| ==> indexes[k] < word.Length
+  invariant forall k :: 0 <= k < |indexes| ==> indexes[k] <= word.Length - query.Length
+  //invariant sorted(indexes, j)
+  decreases word.Length - i
   // j > 0 && j < query.Length && i >= 0 && i < word.Length && w
   // decreases if inRange(i, word.Length, j, query.Length) && word[i] == query[j] then query.Length - j else if inRange(i, word.Length, j, query.Length) &&  word[i] != query[j] && j > 0 then i - word.Length else word.Length - i
   {
     var increment_j := false;
-    if word[i] as char == query[j] {
+    if word[i] == query[j] {
       if j == 0 {
         found := true;  
         pos := i;    
@@ -34,15 +48,16 @@ requires query.Length > 0
       increment_j := true;
     } else if j > 0 {
       var p_j := j;
-      j, found, pos := 0, false, -1;
-    
-      if p_j > 0 && word[i] as char == query[j] {
+      j, found, pos := 0, false, 0;
+      
+      if p_j > 0 && word[i] == query[j] {
         found := true;
         pos := i;
         increment_j := true;
       }
       //i := i - 1;
     } 
+    
     if j == query.Length - 1 {
       if found {
         indexes := indexes + [pos];
@@ -55,8 +70,52 @@ requires query.Length > 0
   }
   
   if !found && |indexes| > 0 {
-    found := true;
+    return true, indexes;
   }
+}
+
+method CastArray(a: array<byte>) returns (chars: array<char>)
+requires a.Length > 0
+ensures fresh(chars)
+ensures a.Length == chars.Length
+ensures forall i :: 0 <= i < a.Length ==> a[i] as char == chars[i]
+
+{
+  chars := new char[a.Length] (i requires 0 <= i < a.Length reads a => a[i] as char);
+}
+
+method BashGrep(word: array<char>, query: array<char>) returns (found: bool, rst: seq<char>)
+requires word.Length > 0
+requires query.Length > 0
+requires word.Length >= query.Length
+{
+  var indexes;
+  found, indexes := Grep(word, query);
+
+  if !found {
+    rst := [];
+    return found, rst;
+  }
+
+  var wordSeq := word[..];
+  rst := [];
+  var i := 0;
+  while i < |indexes| 
+  
+  {
+    var low, high := indexes[i], indexes[i] + query.Length;
+    rst := rst + "<-" + wordSeq[low..high] + "->";
+    if i < |indexes| - 1 {
+      low, high := high, indexes[i + 1];
+      // substituir isto pelo sorted
+      if low < high {
+        rst := rst + wordSeq[low..high];//"...";
+      }
+    }
+    i := i + 1;
+  }
+
+
 }
 
 method {:main} Main(ghost env:HostEnvironment?)
@@ -129,15 +188,29 @@ method {:main} Main(ghost env:HostEnvironment?)
       print "Empty query, exiting.";
       return;
     }
+    var word := CastArray(buffer);
 
-    
-    var found, pos:= Grep(buffer, query);
-    
-    if found {
-     print "YES",", ", pos;
+    print "Word := ", word[..], "\n";
+    print "Query := ", query[..], "\n";
+
+    if word.Length < query.Length {
+      print "File has fewer characters than query string, invalid use! Please add text to the file or query a smaller string.";
+      return;
     }
-    else {
-      print "NO";
+  
+    //var found, pos:= Grep(word, query);
+
+
+    //if found {
+    // print "YES",", ", pos;
+    //}
+    //else {
+    //  print "NO";
+    //}
+    var found, rst := BashGrep(word, query);
+
+    if found {
+      print rst;
     }
 
 }
